AlgoleanTests.lean
@@ -5,6 +5,8 @@ public import AlgoleanTests.ExtendedRealRAMExamples
 public import AlgoleanTests.FreeMonadWP
 public import AlgoleanTests.GaussianAlgorithmsExamples
 public import AlgoleanTests.KMPExamples
+public import AlgoleanTests.MachineExamples
+public import AlgoleanTests.MachineRealRAMExamples
 public import AlgoleanTests.NaivePatternSearchExamples
 public import AlgoleanTests.ProgExamples
 public import AlgoleanTests.QueryExamples
